lib/steel/pulse/Pulse.Syntax.Printer.fst
@@ -502,3 +502,8 @@ let decl_to_string (d:decl) : T.Tac string =
      fst (R.inspect_ident id) ^ " " ^ 
      String.concat " " (T.map (fun (_, b, _) -> binder_to_string b) bs) ^
       " { " ^ st_term_to_string body ^ "}"
+
+  | FnDecl {id; bs} ->
+    "val fn " ^
+     fst (R.inspect_ident id) ^ " " ^
+     String.concat " " (T.map (fun (_, b, _) -> binder_to_string b) bs)
